Sat/Lib/Foldable.lean
@@ -1,9 +1,6 @@
 
 import Sat.Lib.Array
-
--- #check Add
-class One (α : Type u) where
-  one : α
+import Sat.Lib.Monoid
 
 class Foldable (F : Type u → Type v) where
   foldl {α β : Type u} (f : β → α → β) (x₀ : β) (t : F α) : β
@@ -20,34 +17,30 @@ end Foldable
 
 open One
 
-class Monoid (α) extends One α, Mul α where
-  one_mul {x : α} : one * x = x
-  mul_one {x : α} : x * one = x
-  mul_assoc {x y z : α} : (x * y) * z = x * (y * z)
-
-structure MonoidHom (α β) [Monoid α] [Monoid β] where
-  fn : α → β
-  fn_id : fn one = one
-  fn_mul {x y : α} : fn (x * y) = fn x * fn y
-
-instance [Monoid α] [Monoid β] : CoeFun (MonoidHom α β) (λ _ => α → β) where
-  coe f := f.fn
-
-attribute [simp] MonoidHom.fn_id MonoidHom.fn_mul
-
 open Foldable
 class LawfulFoldable (F : Type u → Type v) [Foldable F] where
-  foldl_hom {α β γ : Type u} {f : β → α → β} {g : γ → α → γ} {h : β → γ} {x₀ y₀} (t : F α) :
-    h x₀ = y₀ →
-    (∀ x y, h (f x y) = g (h x) y) →
-    h (foldl f x₀ t) = foldl g y₀ t
+  foldl_sim {α β γ : Type u} {f : β → α → β} {g : γ → α → γ} {SIM : β → γ → Prop} {x₀ y₀} (t : F α) :
+    SIM x₀ y₀ →
+    (∀ a x y, SIM x y → SIM (f x a) (g y a)) →
+    SIM (foldl f x₀ t) (foldl g y₀ t)
 
 namespace LawfulFoldable
+
+variable {F} [Foldable F] [LawfulFoldable F]
+
+theorem foldl_hom {α β γ : Type u} {f : β → α → β} {g : γ → α → γ} {h : β → γ} {x₀ y₀} (t : F α) :
+    h x₀ = y₀ →
+    (∀ x y, h (f x y) = g (h x) y) →
+    h (foldl f x₀ t) = foldl g y₀ t := by
+let R x y := h x = y
+intros h₀ h₁
+apply foldl_sim (SIM := R)
+. assumption
+. simp only; intros; substAll; apply h₁
 
 variable [Monoid α] [Monoid β]
 variable (f : MonoidHom α β)
 
-variable {F} [Foldable F][LawfulFoldable F]
 variable {γ : Type u}
 
 def foldMap_hom (g₀ : γ → α) (x : F γ) :
@@ -56,8 +49,34 @@ apply foldl_hom <;> intros <;> simp
 
 end LawfulFoldable
 
+instance : Foldable List where
+  foldl := List.foldl
+
 instance : Foldable Array where
   foldl := Array.foldl
 
+namespace Array
+
+
+end Array
+
 instance : LawfulFoldable Array where
-  foldl_hom t := Array.foldl_hom _ _ _ _ t
+  foldl_sim :=  by
+    intros; apply Array.foldl_sim <;> auto
+
+namespace List
+
+variable {α β γ : Type u} {f : β → α → β} {g : γ → α → γ} {SIM : β → γ → Prop}
+variable  {x₀ y₀} (t : List α)
+
+theorem foldl_sim :
+    SIM x₀ y₀ →
+    (∀ a x y, SIM x y → SIM (f x a) (g y a)) →
+    SIM (foldl f x₀ t) (foldl g y₀ t) := by
+induction t generalizing x₀ y₀ <;> auto
+
+end List
+
+instance : LawfulFoldable List where
+  foldl_sim :=  by
+    intros; apply List.foldl_sim <;> auto
