Sat/tactics.lean
@@ -27,12 +27,43 @@ macro "left" : tactic =>
 macro "right" : tactic =>
   `(tactic| apply Or.inr)
 
+-- TODO: import mathlib and get rid of this
+syntax "extOrSkip" (ident)* : tactic
+syntax "ext" (ident)* : tactic
+
+macro_rules
+| `(tactic| extOrSkip) => `(tactic| skip)
+| `(tactic| extOrSkip $x $xs) =>
+  `(tactic| apply funext; intro $x; extOrSkip $xs)
+
+macro_rules
+| `(tactic| ext) => `(tactic| repeat (apply funext; intro))
+| `(tactic| ext $xs) =>
+  `(tactic| extOrSkip $xs)
+
+-- syntax "iterate" num tactic : tactic
+-- macro_rules
+-- | `(tactic| iterate 0 $tac) => `(tactic| skip)
+-- | `(tactic| iterate $n $tac) => `(tactic| $tac; iterate $(elabTerm n-1) $tac)
+
+
 namespace Lean.Elab.Tactic
 
 initialize registerTraceClass `refl
+initialize registerTraceClass `substAll
 
 open Expr Lean.Meta
--- #check @Reflexive.refl
+-- #check or
+def applyUnifyAll (g : MVarId) (lmm : Expr) : MetaM (List MVarId) := do
+  let gs ← apply g lmm
+  trace[auto.lemmas]"{gs.length} new goals"
+  trace[auto.lemmas]"types: {(← gs.mapM (inferType ∘ mkMVar))}"
+  trace[auto.lemmas]"types of types: {(← gs.mapM (λ a => do inferType (← inferType $ mkMVar a)))}"
+  guard (← gs.allM λ v => do
+    (← inferType (← inferType (mkMVar v))).isProp)
+  trace[auto.lemmas]"all props"
+  return gs
+
 def tacRefl : TacticM Unit := do
   let g := (← instantiateMVars (← getMainTarget)).consumeMData
   match g with
@@ -45,11 +76,187 @@ def tacRefl : TacticM Unit := do
     trace[refl]"ctorName: {g.ctorName}"
     throwError "Expection a reflexive relation: R x y"
 
+def tacSubstAll : TacticM Unit := do
+  let lctx ← getLCtx
+  trace[substAll] "hyps: {lctx.getFVars}"
+
+  for h in lctx do
+    let t := (← instantiateMVars h.type).consumeMData
+
+    if ¬ h.isAuxDecl then
+      match t with
+      | app (app eq lhs _) rhs _ =>
+        let lc ← getLCtx
+        trace[substAll] "{h.userName} : {t}"
+        if let Option.some _ := lc.find? h.fvarId then
+          trace[substAll] "valid hyp"
+          if eq.isAppOf `Eq ∧ (lhs.isFVar ∨ rhs.isFVar) then
+            trace[substAll] "var eq"
+            liftMetaTactic1 (subst .  h.fvarId)
+          -- else
+            -- pure ()
+            -- trace[substAll] "eq:  {eq.ctorName} {eq}"
+            -- trace[substAll] "lhs: {lhs.ctorName}"
+            -- trace[substAll] "rhs: {rhs.ctorName}"
+        -- else
+            -- trace[substAll] "old"
+      | _ =>
+        trace[substAll] "ignore {h.userName} :  {t.ctorName} {t}"
+
+-- #check apply
+  -- let g := (← instantiateMVars (← getMainTarget)).consumeMData
+  -- match g with
+  -- | (app (app R x _) y _) => liftMetaTactic λ g => do
+  --   let cl ← mkAppOptM ``Reflexive #[none, R]
+  --   let inst ← synthInstance cl
+  --   let reflLmm ← mkAppOptM ``Reflexive.refl #[none, R, inst]
+  --   apply g reflLmm
+  -- | _ =>
+  --   trace[refl]"ctorName: {g.ctorName}"
+  --   throwError "Expection a reflexive relation: R x y"
+
+-- inductive ChoiceTree (σ : Type u) (m : Type u → Type v) : Type u → Type (max (u+1) v)
+-- | empty : ChoiceTree σ m α
+-- | choice {β : Type u} (s : σ) (l : List β) (f : β → m α) : ChoiceTree σ m α
+-- | chain' {β : Type u} : ChoiceTree σ m β → (β → m α) → ChoiceTree σ m α
+-- | push' : ChoiceTree σ m α → ChoiceTree σ m α → ChoiceTree σ m α
+
+-- def ChoiceTree.chain [Bind m] : ChoiceTree σ m β → (β → m α) → ChoiceTree σ m α
+-- | ChoiceTree.empty, _ => ChoiceTree.empty
+-- | ChoiceTree.chain' x f, g => ChoiceTree.chain' x λ a => f a >>= g
+-- | x, f => ChoiceTree.chain' x f
+
+-- def ChoiceTree.push : ChoiceTree σ m α → ChoiceTree σ m α → ChoiceTree σ m α
+-- | ChoiceTree.empty, x => x
+-- | x, ChoiceTree.empty => x
+-- | x, y => ChoiceTree.push' x y
+
+def SearchT (δ : Type u) (m : Type u → Type v) (α : Type u) := (α → m δ) → m δ
+
+namespace SearchT
+
+variable {σ : Type} {m : Type → Type}
+variable {α β : Type}
+
+def pure (x : α) : SearchT δ m α :=
+λ f => f x
+
+def bind (x : SearchT δ m α) (f : α → SearchT δ m β) : SearchT δ m β :=
+λ g => x λ a => f a g
+
+instance : Monad (SearchT δ m) where
+  pure := pure
+  bind := bind
+
+section Alternative
+variable [Alternative m] [Monad m] [MonadBacktrack σ m]
+
+def failure  : SearchT δ m α :=
+λ f => Alternative.failure
+
+def orElse (x : SearchT δ m α) (y : Unit → SearchT δ m α) : SearchT δ m α :=
+λ f => do
+  let s ← saveState
+  Alternative.orElse (x f) λ _ => restoreState s >>= λ _ => y () f
+
+instance : Alternative (SearchT δ m) where
+  failure := failure
+  orElse := orElse
+
+end Alternative
+
+def pick [Alternative m] [Monad m] [MonadBacktrack σ m] (l : List α) : SearchT δ m α :=
+λ g => do
+  let s ← saveState
+  l.firstM λ a => do
+    restoreState s
+    g a
+
+def pick' [Alternative m] [Monad m] [MonadBacktrack σ m] (l : Array α) : SearchT δ m α :=
+λ g => do
+  let s ← saveState
+  l.toList.firstM λ a => do
+    restoreState s
+    g a
+
+instance [Bind m] : MonadLift m (SearchT δ m) where
+  monadLift x f := x >>= f
+
+instance [Bind m] [MonadEnv m] : MonadEnv (SearchT δ m) where
+  getEnv f := getEnv >>= f
+  modifyEnv x f := modifyEnv x >>= f
+
+-- instance [Bind m] [MonadExceptOf ε m] : MonadExceptOf ε (SearchT δ m) where
+--   throw e f := throw e
+--   tryCatch x f g := _
+
+instance [Monad m] [MonadRef m] : MonadRef (SearchT δ m) where
+  getRef f := getRef >>= f
+  withRef s x f := withRef s (x f)
+
+instance [Bind m] [AddErrorMessageContext m] : AddErrorMessageContext (SearchT δ m) where
+  add s m f := AddErrorMessageContext.add s m >>= f
+
+def run [Pure m] (x : SearchT α m α) : m α := x Pure.pure
+
+end SearchT
+
+abbrev SearchTacticM δ := SearchT δ TacticM
+
+namespace SearchTacticM
+
+-- instance [Bind m] : MonadFunctor m (SearchT m) where
+--   monadMap f x δ g := f _
+
+def focus {α : Type} (x : SearchTacticM δ α) : SearchTacticM δ α := do
+  let mvarId :: mvarIds ← getUnsolvedGoals | throwNoGoalsToBeSolved
+  setGoals [mvarId]
+  let a ← x
+  let mvarIds' ← getUnsolvedGoals
+  setGoals (mvarIds' ++ mvarIds)
+  pure a
+
+def focusAndDone {α} (tactic : SearchTacticM δ α) : SearchTacticM δ α :=
+  focus do
+    let a ← tactic
+    done
+    pure a
+
+end SearchTacticM
+
+def isDone : TacticM Bool :=
+Option.isSome <$> optional done
+
+def allGoals [Monad m] [MonadLift TacticM m] (tac : m PUnit) : m PUnit := do
+let gs ← getGoals
+let gs' ← gs.mapM λ g => do setGoals [g]; tac; getGoals
+setGoals gs'.join
+
+def tryTac [Alternative m] [Pure m] (x: m Unit) : m Unit :=
+Alternative.orElse x (λ _ => pure ())
+
+def iterate [Monad m] [MonadLift TacticM m]: Nat → m PUnit → m PUnit
+| 0, _ => pure ()
+| Nat.succ n, tac => do
+  unless (← isDone) do
+    -- tryTac (do
+      ( traceM `auto.iterate s!"iterate n = {n}" : TacticM Unit)
+      tac
+      allGoals $ iterate n tac
+
+def tacMyApply (e : Expr) : TacticM Unit :=
+  liftMetaTactic (applyUnifyAll . e)
+
+-- #check repeat
 end Lean.Elab.Tactic
 
-syntax "refl" : tactic
+-- syntax "refl" : tactic
+open Lean.Elab.Tactic
 
-elab "refl" : tactic => Lean.Elab.Tactic.tacRefl
+elab "apply1" t:term : tactic => withMainContext (do tacMyApply (← elabTerm t none))
+
+elab "refl" : tactic => withMainContext Lean.Elab.Tactic.tacRefl
+elab "substAll" : tactic => withMainContext Lean.Elab.Tactic.tacSubstAll
 
 -- macro "refl" : tactic =>
 --   `(tactic| exact Reflexive.refl _)
@@ -59,7 +266,6 @@ macro "exfalso" : tactic =>
 
 macro "byContradiction" h: ident : tactic =>
   `(tactic| apply Classical.byContradiction; intro h)
-
 
 syntax "trans" (term)? : tactic
 
@@ -161,11 +367,13 @@ open Lean Meta
 --       lemmas
 
 
-
 def getAutoLemmas [Monad m] [MonadEnv m] : m NameSet := do
   -- let n ← getMainModule
   let d := (← autoExtension.getState (← getEnv))
   return d
+    |>.insert ``True.intro
+    |>.insert ``Iff.intro
+    |>.insert ``And.intro
   -- .insert ``True.intro ()
   -- let env ← getEnv
   -- let mut ls : NameSet := NameSet.empty
@@ -178,30 +386,37 @@ def getAutoLemmas [Monad m] [MonadEnv m] : m NameSet := do
   -- return l
 
 initialize registerTraceClass `auto.apply
+initialize registerTraceClass `auto.iterate
 initialize registerTraceClass `auto.apply.attempts
+initialize registerTraceClass `auto.lemmas
 
 open Lean
+
+-- def
 -- @[macro autoAttr] def addAutoLemma : Tactic := fun stx =>
   -- _
 -- #exit
 -- @[macro applyAutoLemma]
-def Meta.applyAuto : TacticM Unit := focusAndDone $ do
-  let apply (n : Name) : TacticM Unit := do
-      trace[auto.apply.attempts] "try {n}"
-      let ls ← Lean.Meta.apply (← getMainGoal) (← mkConstWithLevelParams n)
-      trace[auto.apply] "apply: {n}"
-      -- guard ls.isEmpty <|>
-        -- throwError "no meta variables should remain {ls.length}"
-      replaceMainGoal ls
-  trace[auto.apply]"{(← getAutoLemmas).size} candidates"
-  (← getAutoLemmas).toList.firstM apply
+def Meta.applyAuto : SearchTacticM δ Unit := SearchTacticM.focus $ do
+  let n ← SearchT.pick (← (getAutoLemmas)).toList
+  traceM `auto.lemmas s!"Lemma: {n}"
+  liftMetaTactic (applyUnifyAll . (← (mkConstWithLevelParams n : TacticM _)))
+
+def Meta.applyAssumption : SearchTacticM δ Unit := SearchTacticM.focus $ do
+  let x ← SearchT.pick' (← getLCtx).getFVarIds
+  let lctx ← getLCtx
+  guard (¬ (lctx.get! x).isAuxDecl)
+  traceM `auto.lemmas s!"Hyp: {lctx.get! x |>.userName}"
+  liftMetaTactic (applyUnifyAll . (mkFVar x))
+
+-- #exit
 
 -- attribute [auto] And.intro
 
 elab "#print_auto_db" : command => do
   IO.println (← getAutoLemmas).toList
 
-elab "apply_auto_lemma" : tactic => withMainContext Meta.applyAuto
+-- elab "apply_auto_lemma" : tactic => withMainContext Meta.applyAuto
 
 -- #exit
 -- example : True :=
@@ -233,7 +448,38 @@ def Meta.destructHyp : TacticM Unit := focus $ do
   guard changed
   -- return ()
 
+section HOrElse
+variable  [Alternative m] [Monad m] [MonadBacktrack σ m]
+instance : HOrElse (m α) (SearchT δ m α) (SearchT δ m α) where
+  hOrElse x y := (Alternative.orElse (liftM x) y)
+
+instance : HOrElse (SearchT δ m α) (m α) (SearchT δ m α) where
+  hOrElse x y := (Alternative.orElse x (liftM ∘ y))
+
+end HOrElse
+
+-- def traceState
+
+def withMainContext' (x : SearchTacticM δ α) : SearchTacticM δ α :=
+λ f => withMainContext (x f)
+
+def Meta.tacAutoStep : SearchTacticM δ Unit :=
+withMainContext' $
+  Lean.Elab.Tactic.tacRefl <|>
+  Meta.applyAssumption <|>
+  Meta.destructHyp <|>
+  liftMetaTactic1 ((some ∘ Prod.snd) <$> intro1 .) <|>
+  Meta.applyAuto
+  -- (do let g ← getMainGoal; (throwError "do {(← ppGoal g)}") : TacticM Unit)
+
+def Meta.tacAuto : SearchTacticM δ Unit :=
+SearchTacticM.focusAndDone $
+iterate 10 Meta.tacAutoStep
+
 elab "destruct_hyp" : tactic => withMainContext Meta.destructHyp
+elab "auto" : tactic => withMainContext Meta.tacAuto.run
+elab "auto_step" : tactic => withMainContext Meta.tacAutoStep.run
+elab "apply_auto" : tactic => withMainContext Meta.applyAuto.run
 
   -- destruct_hyp
 
@@ -242,31 +488,31 @@ elab "destruct_hyp" : tactic => withMainContext Meta.destructHyp
 -- #exit
 initialize registerTraceClass `auto
 
-macro "auto" : tactic =>
-  `(tactic|
-    solve
-    | repeat
-        first
-        | refl
-        | apply True.intro
-        | assumption
-        | destruct_hyp
-        | apply And.intro
-        | apply Iff.intro
-        | intros _
-        | apply_auto_lemma )
+-- macro "auto" : tactic =>
+--   `(tactic|
+--     solve
+--     | repeat
+--         first
+--         | refl
+--         | apply True.intro
+--         | assumption
+--         | destruct_hyp
+--         | apply And.intro
+--         | apply Iff.intro
+--         | intros _
+--         | apply_auto_lemma )
 
-macro "auto_step" : tactic =>
-  `(tactic|
-        first
-        | refl
-        | apply True.intro
-        | assumption
-        | destruct_hyp
-        | apply And.intro
-        | apply Iff.intro
-        | intros _
-        | apply_auto_lemma )
+-- macro "auto_step" : tactic =>
+--   `(tactic|
+--         first
+--         | refl
+--         | apply True.intro
+--         | assumption
+--         | destruct_hyp
+--         | apply And.intro
+--         | apply Iff.intro
+--         | intros _
+--         | apply_auto_lemma )
 
 -- theorem swapHyp {p q : Prop} (h : p) (h' : ¬ p) : q := by
 --   cases h' h
